proof/old_system/uni/algo_worklist/prop_soundness.v
@@ -11,6 +11,7 @@ Require Import uni.decl.prop_typing.
 Require Import uni.decl_worklist.prop_equiv.
 Require Import uni.algo_worklist.def_extra.
 Require Import uni.algo_worklist.prop_basic.
+Require Import uni.algo_worklist.prop_rename.
 Require Import uni.algo_worklist.transfer.
 Require Import ln_utils.
 
@@ -1282,7 +1283,6 @@ Proof with eauto.
     destruct_trans. rename_typ.
     exists (work_infer (exp_var_f x) csᵈ ⫤ᵈ Ω).
     split... exists θ. econstructor... econstructor...
-    admit. (* *, binds *)
     admit. (* *, uniq *) 
   (* e : A => _ *)
   - exists (work_infer (exp_anno eᵈ Aᵈ) csᵈ ⫤ᵈ Ω)...
